upgrade lean; lr for mut states

lean/STLC/STLC/Env.lean
@@ -25,6 +25,10 @@ lemma indexrSome' : ∀ {A} (xs : List A) i,
     . simp [if_neg h'] at h; simp;
       have h' := ih h; omega
 
+lemma indexrSome'' : ∀ {A} (xs : List A) i,
+  (∃ x, indexr i xs = some x) → (¬i = xs.length) := by
+  intros A xs i h; have h'' := indexrSome' _ _ h; omega
+
 lemma indexrHead : ∀ {A} (x : A) (xs : List A),
   indexr xs.length (x :: xs) = some x := by intros A x xs; simp
 
@@ -34,3 +38,40 @@ lemma indexrNone : ∀ {A} (xs : List A) i,
   case cons x xs ih =>
     simp at h; have h' : ¬ i = xs.length := by omega
     rw [if_neg h']; apply ih; omega
+
+lemma indexrSkip : ∀ {A} (x: A) (xs : List A) i,
+  (¬i = xs.length) → indexr i (x :: xs) = indexr i xs := by
+  intros A x xs i h; simp; intros h'; omega
+
+@[simp]
+def update {X : Type} (l : List X) (n : ℕ) (x : X) : List X :=
+  match l with
+  | [] => []
+  | a :: l' => if n == l'.length then x :: l' else a :: update l' n x
+
+lemma updateLength : ∀ {A} (xs : List A) i x,
+  xs.length = (update xs i x).length := by
+  intros A xs i x; induction xs <;> simp
+  case cons y ys ih =>
+    by_cases h': i = ys.length
+    . subst h'; simp
+    . simp [if_neg h']; apply ih
+
+lemma indexrUpdateHit : ∀ {A} (x : A) (xs : List A) i,
+  i < xs.length → indexr i (update xs i x) = some x := by
+  intros A x xs i h; induction xs <;> simp at h
+  case cons y ys ih =>
+    by_cases h': i = ys.length
+    . subst h'; simp
+    . simp [if_neg h']; simp [<- updateLength]; simp [if_neg h']
+      apply ih; omega
+
+lemma indexrUpdateMiss : ∀ {A} (xs : List A) i x j,
+  j ≠ i → indexr j (update xs i x) = indexr j xs := by
+  intros A xs i x j hij; induction xs <;> simp
+  case cons y ys ih =>
+    by_cases h': i = ys.length <;> by_cases h'' : j = ys.length
+    . omega
+    . rw [h', if_neg h'']; simp; intro; omega
+    . rw [if_neg h', h'']; simp; intro hu; rw [<- updateLength] at hu; omega
+    . rw [if_neg h', if_neg h'']; simp; rw [<- updateLength]; rw [if_neg h'']; apply ih
