lean/STLC/STLC/Smallstep_Ref_Equiv.lean
@@ -1,0 +1,623 @@
+-- STLC
+-- locally nameless where free variables are de Bruijn levels
+-- first-order reference store
+-- call-by-value small-step semantics and binary logical relations
+-- contextual equivalence
+
+import Mathlib.Data.Finset.Sort
+import STLC.Env
+
+namespace Smallstep_Ref_Equiv
+
+inductive ty : Type
+| bool : ty
+| ref : ty → ty
+| arrow : ty → ty → ty
+
+inductive tm : Type
+| fls : tm
+| tru : tm
+| bvar : ℕ → tm
+| fvar : ℕ → tm
+| abs : tm → tm
+| app : tm → tm → tm
+| loc : ℕ → tm
+| ref : tm → tm
+| deref : tm → tm
+| assign : tm → tm → tm
+
+abbrev tenv := List ty
+abbrev venv := List tm
+
+-- combine open and subst: t1[n ↦ t2]
+@[simp]
+def openSubst (t1: tm) (n: ℕ) (t2: tm) : tm :=
+  match t1 with
+  | .fls | .tru => t1
+  | .bvar x =>
+    if x = n then t2
+    -- else if n < x then .bvar (x - 1)
+    else .bvar x
+  | .fvar x => .fvar x
+  | .abs t1 => .abs (openSubst t1 (n + 1) t2)
+  | .app t11 t12 =>
+    .app (openSubst t11 n t2) (openSubst t12 n t2)
+  | .loc x => .loc x
+  | .ref t1 => .ref (openSubst t1 n t2)
+  | .deref t1 => .deref (openSubst t1 n t2)
+  | .assign t11 t12 => .assign (openSubst t11 n t2) (openSubst t12 n t2)
+
+@[simp]
+def close (t1: tm) (n: ℕ) (m: ℕ) : tm :=
+  match t1 with
+  | .fls | .tru => t1
+  | .bvar x => .bvar x
+  | .fvar x => if x = n then (.bvar m) else t1
+  | .abs t1 => .abs (close t1 n (m + 1))
+  | .app t11 t12 =>
+    .app (close t11 n m) (close t12 n m)
+  | .loc x => .loc x
+  | .ref t1 => .ref (close t1 n m)
+  | .deref t1 => .deref (close t1 n m)
+  | .assign t1 t2 => .assign (close t1 n m) (close t2 n m)
+
+@[simp]
+def substF (Δ: venv) (t: tm) : tm :=
+  match t with
+  | .fls | .tru => t
+  | .bvar _ => t
+  | .fvar x =>
+    match indexr x Δ with
+    | none => t
+    | some t' => t'
+  | .abs t1 => .abs (substF Δ t1)
+  | .app t11 t12 => .app (substF Δ t11) (substF Δ t12)
+  | .loc x => .loc x
+  | .ref t1 => .ref (substF Δ t1)
+  | .deref t1 => .deref (substF Δ t1)
+  | .assign t1 t2 => .assign (substF Δ t1) (substF Δ t2)
+
+@[simp]
+def closedF (t: tm) (n: ℕ) : Prop :=
+  match t with
+  | .fls | .tru => true
+  | .bvar _ => true
+  | .fvar x => x < n
+  | .abs t1 => closedF t1 n
+  | .app t11 t12 => closedF t11 n ∧ closedF t12 n
+  | .loc _ => true
+  | .ref t1 => closedF t1 n
+  | .deref t1 => closedF t1 n
+  | .assign t1 t2 => closedF t1 n ∧ closedF t2 n
+
+@[simp]
+def closedB (t: tm) (n: ℕ) : Prop :=
+  match t with
+  | .fls | .tru => true
+  | .bvar x => x < n
+  | .fvar _ => true
+  | .abs t1 => closedB t1 (n + 1)
+  | .app t11 t12 => closedB t11 n ∧ closedB t12 n
+  | .loc _ => true
+  | .ref t1 => closedB t1 n
+  | .deref t1 => closedB t1 n
+  | .assign t1 t2 => closedB t1 n ∧ closedB t2 n
+
+@[simp]
+def closedL (t: tm) (n: ℕ) : Prop :=
+  match t with
+  | .fls | .tru => true
+  | .bvar _ => true
+  | .fvar _ => true
+  | .abs t1 => closedL t1 n
+  | .app t11 t12 => closedL t11 n ∧ closedL t12 n
+  | .loc x => x < n
+  | .ref t1 => closedL t1 n
+  | .deref t1 => closedL t1 n
+  | .assign t1 t2 => closedL t1 n ∧ closedL t2 n
+
+lemma openClosed : ∀ t n m,
+  closedB (openSubst t m (.fvar n)) m →
+  closedB t (m+1) := by
+  intros t; induction t <;> intros n m h <;> simp
+  case bvar x =>
+    by_cases hx: (x = m)
+    . omega
+    . by_cases hx': (x < m)
+      omega; unfold openSubst at h;
+      rw [if_neg hx] at h; have hx'' : (m < x) := by omega;
+      simp [hx''] at h; omega
+  case abs t ih =>
+    apply ih n (m+1); unfold openSubst at h; simp at h; assumption
+  case app t1 t2 ih1 ih2 =>
+    apply And.intro; apply ih1 n m h.1; apply ih2 n m h.2
+  case ref t ih =>
+    apply ih n m h
+  case deref t ih =>
+    apply ih n m h
+  case assign t1 t2 ih1 ih2 =>
+    simp at h; apply And.intro; apply ih1 n m h.1; apply ih2 n m h.2
+
+lemma openClosed': ∀ t n m,
+    closedB t (m+1) → closedB (openSubst t m (.fvar n)) m := by
+  intros t; induction t <;> intros n m h <;> simp
+  case bvar x =>
+    by_cases hx: (x = m)
+    . simp [hx]
+    . rw [if_neg hx]; simp at h; simp; omega
+  case abs t ih =>
+    apply ih n (m+1); simp at h; assumption
+  case app t1 t2 ih1 ih2 =>
+    apply And.intro; apply ih1 n m h.1; apply ih2 n m h.2
+  case ref t ih =>
+    apply ih n m h
+  case deref t ih =>
+    apply ih n m h
+  case assign t1 t2 ih1 ih2 =>
+    simp at h; apply And.intro; apply ih1 n m h.1; apply ih2 n m h.2
+
+lemma closedBOpenId: ∀ t1 t2 n,
+  closedB t1 n -> openSubst t1 n t2 = t1 := by
+  intros t1; induction t1 <;> intros t2 n h <;> simp
+  case bvar x => intros hxn; simp at h; omega
+  case abs t ih => simp at h; apply ih; assumption
+  case app t1 t2 ih1 ih2 =>
+    apply And.intro
+    . apply ih1; apply h.1
+    . apply ih2; apply h.2
+  case ref t ih => apply ih; apply h
+  case deref t ih => apply ih; apply h
+  case assign t1 t2 ih1 ih2 =>
+    simp at h; apply And.intro
+    . apply ih1; apply h.1
+    . apply ih2; apply h.2
+
+lemma closedBInc: ∀ t n n1,
+    closedB t n -> n <= n1 -> closedB t n1 := by
+  intros t; induction t <;> intros n n1 hcl hle <;> simp
+  case bvar x => simp at hcl; omega
+  case abs t ih => simp at hcl; apply ih; apply hcl; omega
+  case app t1 t2 ih1 ih2 =>
+    apply And.intro
+    . apply ih1; apply hcl.1; omega
+    . apply ih2; apply hcl.2; omega
+  case ref t ih => apply ih; apply hcl; omega
+  case deref t ih => apply ih; apply hcl; omega
+  case assign t1 t2 ih1 ih2 =>
+    simp at hcl; apply And.intro
+    . apply ih1; apply hcl.1; omega
+    . apply ih2; apply hcl.2; omega
+
+lemma closedFInc: ∀ t n k, closedF t n -> closedF (openSubst t k (tm.fvar n)) (n + 1) := by
+  intros t; induction t <;> intros n k hcl <;> simp
+  case fvar x => simp at hcl; omega
+  case bvar x =>
+    by_cases hx: (x = k)
+    . simp [hx];
+    . rw [if_neg hx]; simp;
+  case abs t ih => apply ih; simp at hcl; assumption
+  case app t1 t2 ih1 ih2 =>
+    apply And.intro
+    . apply ih1; apply hcl.1
+    . apply ih2; apply hcl.2
+  case ref t ih => apply ih; apply hcl
+  case deref t ih => apply ih; apply hcl
+  case assign t1 t2 ih1 ih2 =>
+    simp at hcl; apply And.intro
+    . apply ih1; apply hcl.1
+    . apply ih2; apply hcl.2
+
+lemma substFOpenComm : ∀ t t1 Δ n, closedF t Δ.length →
+  (∀ x t1, indexr x Δ = some t1 → closedB t1 0) →
+  substF (t1::Δ) (openSubst t n (.fvar Δ.length)) =
+  openSubst (substF Δ t) n t1 := by
+  intros t t1 Δ n h; revert n; induction t <;> intros n hc <;> simp
+  case bvar x =>
+    by_cases hx: (x = n)
+    . simp [hx]
+    . rw [if_neg hx]; rw [if_neg hx]; simp
+  case fvar x =>
+    have h' := indexrSome Δ x h
+    rcases h' with ⟨v, hidx⟩; rw [hidx]; simp;
+    have hx : ¬(x = Δ.length) := by simp at h; omega
+    rw [if_neg hx]; simp;
+    rw [closedBOpenId]; apply closedBInc; apply hc; apply hidx; omega
+  case abs t ih => apply ih; simp at h; assumption; apply hc
+  case app t1 t2 ih1 ih2 =>
+    simp at h; apply And.intro
+    . apply ih1; apply h.1; assumption
+    . apply ih2; apply h.2; assumption
+  case ref t ih =>
+    simp at h; apply ih; apply h; assumption
+  case deref t ih =>
+    simp at h; apply ih; apply h; assumption
+  case assign t1 t2 ih1 ih2 =>
+    simp at h; apply And.intro
+    . apply ih1; apply h.1; assumption
+    . apply ih2; apply h.2; assumption
+
+lemma substFClosedBComm: ∀ t Δ n,
+  (forall x t1, indexr x Δ = some t1 -> closedB t1 0) ->
+  (closedB t n) -> (closedB (substF Δ t) n) := by
+  intros t; induction t <;> intros E n hidx hcl <;> simp
+  case bvar x => simp at hcl; assumption
+  case fvar x =>
+    generalize h : indexr x E = v
+    cases v <;> simp
+    case some v => apply closedBInc; apply hidx; apply h; omega
+  case abs t ih => apply ih; apply hidx; simp at hcl; assumption
+  case app t1 t2 ih1 ih2 =>
+    rcases hcl with ⟨hcl1, hcl2⟩
+    apply And.intro
+    . apply ih1; apply hidx; assumption
+    . apply ih2; apply hidx; assumption
+  case ref t ih => apply ih; apply hidx; assumption
+  case deref t ih => apply ih; apply hidx; assumption
+  case assign t1 t2 ih1 ih2 =>
+    rcases hcl with ⟨hcl1, hcl2⟩
+    apply And.intro
+    . apply ih1; apply hidx; assumption
+    . apply ih2; apply hidx; assumption
+
+@[simp]
+def binds x τ (Γ : tenv) := (indexr x Γ = some τ)
+
+abbrev stty := List ty -- Φ, restricted to List .bool
+
+inductive hasType : stty → tenv → tm → ty → Prop
+| fls : ∀ Φ Γ, hasType Φ Γ .fls .bool
+| tru : ∀ Φ Γ, hasType Φ Γ .tru .bool
+| var : ∀ Φ Γ x τ, binds x τ Γ → hasType Φ Γ (.fvar x) τ
+| abs : ∀ Φ Γ t τ₁ τ₂,
+  hasType Φ (τ₁::Γ) (openSubst t 0 (.fvar Γ.length)) τ₂ →
+  closedF t Γ.length →
+  hasType Φ Γ (.abs t) (ty.arrow τ₁ τ₂)
+| app : ∀ Φ Γ t₁ t₂ τ₁ τ₂,
+  hasType Φ Γ t₁ (.arrow τ₁ τ₂) →
+  hasType Φ Γ t₂ τ₁ →
+  hasType Φ Γ (.app t₁ t₂) τ₂
+| loc : ∀ Φ Γ n,
+  n < Φ.length →
+  hasType Φ Γ (.loc n) (.ref .bool)
+| ref : ∀ Φ Γ t,
+  hasType Φ Γ t (.bool) →
+  hasType Φ Γ (.ref t) (.ref .bool)
+| deref : ∀ Φ Γ t τ,
+  hasType Φ Γ t (.ref τ) →
+  hasType Φ Γ (.deref t) τ
+| assign : ∀ Φ Γ t₁ t₂ τ,
+  hasType Φ Γ t₁ (.ref τ) →
+  hasType Φ Γ t₂ τ →
+  hasType Φ Γ (.assign t₁ t₂) .bool -- for simplicity, we use bool for the result, could be unit
+
+inductive value : tm → Prop
+| fls : value .fls
+| tru : value .tru
+| loc : ∀ n, value (.loc n)
+| abs : ∀ t, value (.abs t)
+
+abbrev st := List tm
+
+inductive step : st → tm → st → tm → Prop
+| beta : ∀ σ t v,
+  value v →
+  step σ (.app (.abs t) v) σ (openSubst t 0 v)
+| app1 : ∀ σ σ' t1 t1' t2,
+  step σ t1 σ' t1' →
+  step σ (.app t1 t2) σ' (.app t1' t2)
+| app2 : ∀ σ σ' t1 t2 t2',
+  value t1 →
+  step σ t2 σ' t2' →
+  step σ (.app t1 t2) σ' (.app t1 t2')
+| ref_val : ∀ σ v,
+  value v →
+  step σ (.ref v) (v::σ) (.loc (σ.length))
+| ref : ∀ σ σ' t t',
+  step σ t σ' t' →
+  step σ (.ref t) σ' (.ref t')
+| deref_val : ∀ σ n v,
+  indexr n σ = some v →
+  step σ (.deref (.loc n)) σ v
+| deref : ∀ σ σ' t t',
+  step σ t σ' t' →
+  step σ (.deref t) σ' (.deref t')
+| assign_val : ∀ σ n v,
+  n < σ.length →
+  value v →
+  step σ (.assign (.loc n) v) (update σ n v) v
+| assign1 : ∀ σ σ' t1 t1' t2,
+  step σ t1 σ' t1' →
+  step σ (.assign t1 t2) σ' (.assign t1' t2)
+| assign2 : ∀ σ σ' t1 t2 t2',
+  value t1 →
+  step σ t2 σ' t2' →
+  step σ (.assign t1 t2) σ' (.assign t1 t2')
+
+inductive stepn : st → tm → st → tm → Prop
+| refl : ∀ σ t, stepn σ t σ t
+| multi : ∀ σ1 σ2 σ3 t1 t2 t3, stepn σ1 t1 σ2 t2 → step σ2 t2 σ3 t3 → stepn σ1 t1 σ3 t3
+
+lemma stepnApp1 : ∀ σ1 σ2 t1 t1' t2,
+  stepn σ1 t1 σ2 t1' → stepn σ1 (.app t1 t2) σ2 (.app t1' t2) := by
+  intros σ1 σ2 t1 t1' t2 h; induction h
+  . constructor
+  . case _ hstn hst ih => constructor; assumption; apply step.app1; assumption
+
+lemma stepnApp2 : ∀ σ1 σ2 t1 t2 t2',
+  value t1 → stepn σ1 t2 σ2 t2' → stepn σ1 (.app t1 t2) σ2 (.app t1 t2') := by
+  intros σ1 σ2 t1 t2 t2' hv h; induction h
+  . constructor
+  . case _ hstn hst ih => apply stepn.multi; assumption; apply step.app2; assumption; assumption
+
+lemma stepnRef : ∀ σ1 σ2 t1 t2,
+  stepn σ1 t1 σ2 t2 → stepn σ1 (.ref t1) σ2 (.ref t2) := by
+  intros σ1 σ2 t1 t2 h; induction h
+  . constructor
+  . case _ hstn hst ih => constructor; assumption; apply step.ref; assumption
+
+lemma stepnRefVal : ∀ σ1 v,
+  value v → stepn σ1 (.ref v) (v::σ1) (.loc (σ1.length)) := by
+  intros σ1 v hv; apply stepn.multi; apply stepn.refl;
+  apply step.ref_val; assumption
+
+lemma stepnTrans : ∀ σ1 σ2 σ3 t1 t2 t3, stepn σ1 t1 σ2 t2 → stepn σ2 t2 σ3 t3 → stepn σ1 t1 σ3 t3 := by
+  intros σ1 σ2 σ3 t1 t2 t3 h1 h2; induction h2
+  . assumption
+  . case _ _ _ _ _ _ hstn hst ih =>
+    apply stepn.multi; apply ih; assumption; assumption
+
+-- the "world"
+@[simp]
+def st_rel := ℕ → ℕ → Prop
+
+@[simp]
+def st_rel.mt : st_rel := fun _ _ => false
+
+@[simp]
+def st_rel.ext (m: st_rel) (a b: ℕ): st_rel :=
+  fun x y => (x = a ∧ y = b) ∨ (¬ x = a ∧ ¬ y = b ∧ m x y)
+
+-- extend the "world"
+@[simp]
+def extend (m1 m2 : st_rel) : Prop := ∀ a b, m1 a b → m2 a b
+
+notation:60 a:65 "≥" b:65 => extend a b
+
+@[simp]
+def bijection {X Y} (f: X → Y → Prop): Prop :=
+  (∀ x y y', f x y → f x y' → y = y') ∧ (∀ x x' y, f x y → f x' y → x = x')
+
+@[simp]
+def storeType (σ1 σ2 : st) (m : st_rel) : Prop :=
+  (∀ l1 l2, m l1 l2 → ∃ v, indexr l1 σ1 = some v ∧ indexr l2 σ2 = some v) ∧ bijection m
+
+@[simp]
+def valType (m: st_rel) (t1 : tm) (t2 : tm) (τ : ty) : Prop :=
+  match t1, t2, τ with
+  | .fls, .fls, .bool => true
+  | .tru, .tru, .bool => true
+  | .loc n1, .loc n2, .ref τ => m n1 n2
+  | (.abs t1), (.abs t2), .arrow τ1 τ2 =>
+    ∀ v1 v2 m1 st1 st2,
+    m ≥ m1 →
+    storeType st1 st2 m1 →
+    valType m1 v1 v2 τ1 → closedB v1 0 → closedB v2 0 →
+    ∃ v3 v4 m2 st1' st2',
+    m1 ≥ m2 →
+    storeType st1' st2' m2 →
+    stepn st1 (openSubst t1 0 v1) st1' v3 ∧ closedB v3 0 ∧
+    stepn st2 (openSubst t2 0 v2) st2' v4 ∧ closedB v4 0 ∧
+    valType m2 v3 v4 τ2
+  | _, _, _ => false
+
+@[simp]
+def expType (st1 st2 : st) (m : st_rel) (t1 t2 : tm) (τ : ty) : Prop :=
+  ∃ st1' st2' m' v1 v2,
+    m ≥ m' ∧
+    storeType st1' st2' m' ∧
+    stepn st1 t1 st1' v1 ∧
+    stepn st2 t2 st2' v2 ∧
+    closedB v1 0 ∧ closedB v2 0 ∧
+    valType m' v1 v2 τ
+
+@[simp]
+def envType (m : st_rel) (Δ1 : venv) (Δ2 : venv) (Γ : tenv) : Prop :=
+  Δ1.length = Γ.length ∧
+  Δ2.length = Γ.length ∧
+  ∀ τ x, binds x τ Γ →
+  ∃ v1 v2,
+  indexr x Δ1 = some v1 ∧ closedB v1 0 ∧
+  indexr x Δ2 = some v2 ∧ closedB v2 0 ∧
+  valType m v1 v2 τ
+
+@[simp]
+def wf (t: tm) (Γ: tenv) := closedB t 0 ∧ closedF t (Γ.length)
+
+@[simp]
+def semType (Γ : tenv) (t1 t2 : tm) (τ : ty) : Prop :=
+  ∀ st1 st2 m Δ1 Δ2,
+  wf t1 Γ → wf t2 Γ →
+  envType m Δ1 Δ2 Γ →
+  storeType st1 st2 m →
+  expType st1 st2 m (substF Δ1 t1) (substF Δ2 t2) τ
+
+lemma valTypeValue : ∀ m t1 t2 τ, valType m t1 t2 τ → value t1 ∧ value t2 := by
+  intros m t1 t2 τ h; cases t1 <;> cases t2 <;> try simp at h
+  . apply And.intro <;> constructor
+  . apply And.intro <;> constructor
+  . next t1 t2 => apply And.intro <;> apply value.abs
+  . apply And.intro <;> constructor
+
+lemma extend.refl : ∀ m, m ≥ m := by intros m a b h; assumption
+
+lemma extend.ext : ∀ st1 st2 m,
+  storeType st1 st2 m →
+  m ≥ (st_rel.ext m st1.length st2.length) :=
+  by
+  intros st1 st2 m h; simp;
+  intros a b h'; right; rcases h with ⟨h1, h2⟩;
+  specialize h1 _ _ h'; rcases h1 with ⟨v, hidx1, hidx2⟩;
+  apply And.intro; apply indexrSome'' _ _ ⟨v, hidx1⟩
+  apply And.intro; apply indexrSome'' _ _ ⟨v, hidx2⟩
+  assumption
+
+lemma extend.trans : ∀ {m1 m2 m3},
+  m1 ≥ m2 → m2 ≥ m3 → m1 ≥ m3 := by
+  intros m1 m2 m3 h12 h23 a b h; apply h23; apply h12; assumption
+
+lemma envType.empty : envType st_rel.mt [] [] [] := by simp
+
+lemma envType.extend : ∀ m Δ1 Δ2 Γ v1 v2 τ,
+  envType m Δ1 Δ2 Γ →
+  closedB v1 0 → closedB v2 0 →
+  valType m v1 v2 τ →
+  envType m (v1::Δ1) (v2::Δ2) (τ::Γ) := by
+  intros m Δ1 Δ2 Γ v1 v2 τ henv hclv1 hclv2 hv12
+  constructor; simp; apply henv.1
+  constructor; simp; apply henv.2.1
+  intros τ' x hbd; rcases henv with ⟨hlen1, hlen2, h⟩
+  by_cases hx: (x = Δ1.length)
+  . simp [hx]; constructor; assumption; simp [hlen1, hlen2]
+    constructor; assumption; simp at hbd; simp [hx, hlen1] at hbd
+    rw [<- hbd]; assumption
+  . simp at hbd; rw [<-hlen1, if_neg hx] at hbd;
+    simp; rw [if_neg hx]; rw [hlen2, <-hlen1, if_neg hx]
+    specialize h τ' x hbd; rcases h with ⟨v1, v2, h⟩
+    exists v1; constructor; exact h.1; constructor; exact h.2.1
+    exists v2; exact h.2.2
+
+lemma envType.closed : ∀ m Δ1 Δ2 Γ, envType m Δ1 Δ2 Γ →
+  (∀ x t1, indexr x Δ1 = some t1 → closedB t1 0) ∧
+  (∀ x t1, indexr x Δ2 = some t1 → closedB t1 0) := by
+  intros m Δ1 Δ2 Γ henv; rcases henv with ⟨hlen1, hlen2, h⟩
+  apply And.intro
+  . intros x t1 hidx;
+    have hx : (x < Δ1.length) := by apply indexrSome'; exists t1
+    rw [hlen1] at hx; have hidx' := indexrSome Γ x hx
+    rcases hidx' with ⟨τ, hidx'⟩;
+    have ⟨v1, v2, hidxv1, hclv1, hidxv2, hclv2, hval⟩  := h τ x hidx'
+    rw [hidx] at hidxv1; cases hidxv1; assumption
+  . intros x t1 hidx;
+    have hx : (x < Δ2.length) := by apply indexrSome'; exists t1
+    rw [hlen2] at hx; have hidx' := indexrSome Γ x hx
+    rcases hidx' with ⟨τ, hidx'⟩;
+    have ⟨v1, v2, hidxv1, hclv1, hidxv2, hclv2, hval⟩  := h τ x hidx'
+    rw [hidx] at hidxv2; cases hidxv2; assumption
+
+lemma storeType.mt : storeType [] [] st_rel.mt := by
+  constructor; intros l1 l2 h; cases h; simp
+
+lemma storeType.ext : ∀ σ1 σ2 m v1 v2,
+  storeType σ1 σ2 m →
+  valType m v1 v2 .bool →
+  storeType (v1::σ1) (v2::σ2) (st_rel.ext m σ1.length σ2.length) := by
+  intros σ1 σ2 m v1 v2 hst hv12
+  rcases hst with ⟨h1, h2⟩
+  apply And.intro
+  . intros l1 l2 m'; cases m' with
+    | inl h =>
+      rcases h with ⟨hidx1, hidx2⟩
+      rw [hidx1, hidx2]; rw [indexrHead]; rw [indexrHead]
+      cases v1 <;> cases v2 <;> simp at hv12
+      exists .fls; exists .tru
+    | inr h =>
+      specialize h1 l1 l2 h.2.2
+      rcases h1 with ⟨v, hidx1, hidx2⟩
+      exists v; rw [indexrSkip, indexrSkip]; aesop; aesop; aesop
+  . rcases h2 with ⟨h21, h22⟩; aesop
+
+lemma storeType.update : ∀ st1 st2 m v1 v2 l1 l2,
+  storeType st1 st2 m →
+  valType m v1 v2 .bool →
+  m l1 l2 →
+  storeType (update st1 l1 v1) (update st2 l2 v2) (st_rel.ext m l1 l2) := by
+  intros st1 st2 m v1 v2 l1 l2 hst hv12 hm
+  rcases hst with ⟨h1, h2⟩
+  apply And.intro
+  . intros l1' l2' m'
+    by_cases h': l1 = l1' <;> by_cases h'': l2 = l2' <;> simp [h', h''] at m' <;> try omega
+    . subst h'; subst h''
+      specialize h1 l1 l2 hm; rcases h1 with ⟨v, hidx1, hidx2⟩
+      rw [indexrUpdateHit]; rw [indexrUpdateHit]
+      cases v1 <;> cases v2 <;> simp at hv12; exists .fls; exists .tru
+      apply indexrSome'; exists v; apply indexrSome'; exists v
+    . cases m' with
+      | inl h => aesop
+      | inr h =>
+        specialize h1 l1' l2' h.2.2
+        rcases h1 with ⟨v, hidx1, hidx2⟩
+        exists v; rw [indexrUpdateMiss]; rw [indexrUpdateMiss];
+        apply And.intro <;> assumption; omega; omega
+  . rcases h2 with ⟨h21, h22⟩; aesop
+
+lemma valType.antimono : ∀ m1 m2 v1 v2 τ,
+  valType m1 v1 v2 τ → m1 ≥ m2 → valType m2 v1 v2 τ := by
+  intros m1 m2 v1 v2 τ hv12 hm;
+  cases v1 <;> cases v2 <;> try simp at hv12
+  . cases τ <;> try simp at hv12 <;> simp
+  . cases τ <;> try simp at hv12 <;> simp
+  . cases τ; simp at hv12; simp at hv12
+    next t1 t2 τ1 τ2 =>
+    intros v3 v4 m3 st1 st2 hm'
+    specialize hv12 v3 v4 m3 st1 st2 (extend.trans hm hm'); assumption
+  . cases τ <;> try simp at hv12 <;> aesop
+
+lemma envType.antimono : ∀ m1 m2 Δ1 Δ2 Γ,
+  envType m1 Δ1 Δ2 Γ → m1 ≥ m2 → envType m2 Δ1 Δ2 Γ := by
+  intros m1 m2 Δ1 Δ2 Γ henv hm; rcases henv with ⟨hlen1, hlen2, h⟩
+  constructor; aesop; constructor; aesop
+  intros τ x hbd; rcases h τ x hbd with ⟨v1, v2, hidxv1, hclv1, hidxv2, hclv2, hv12⟩
+  specialize h τ x hbd; aesop; apply valType.antimono; apply hv12; apply hm
+
+-- compatibility lemmas
+
+lemma semTrue : ∀ Γ, semType Γ .tru .tru .bool := by
+  intros Γ st1 st2 m Δ1 Δ2 _ _ _ _;
+  exists st1, st2, m, .tru, .tru;
+  apply And.intro; apply extend.refl; apply And.intro; assumption;
+  simp; apply And.intro <;> apply stepn.refl
+
+lemma semFalse : ∀ Γ, semType Γ .fls .fls .bool := by
+  intros Γ st1 st2 m Δ1 Δ2 _ _ _ _;
+  exists st1, st2, m, .fls, .fls;
+  apply And.intro; apply extend.refl; apply And.intro; assumption;
+  simp; apply And.intro <;> apply stepn.refl
+
+lemma semVar : ∀ Γ x τ, binds x τ Γ → semType Γ (.fvar x) (.fvar x) τ := by
+  intros Γ x τ hbd st1 st2 m Δ1 Δ2 _ _ henv hst
+  rcases henv with ⟨_, _, h⟩
+  have ⟨v1, v2, idx1, cl1, idx2, cl2, semv⟩ := h τ x hbd
+  exists st1, st2, m, v1, v2; simp [idx1, idx2]
+  apply And.intro; apply hst
+  exact ⟨stepn.refl st1 v1, stepn.refl st2 v2, cl1, cl2, semv⟩
+
+lemma semRef : ∀ Γ t1 t2,
+  semType Γ t1 t2 .bool →
+  semType Γ (.ref t1) (.ref t2) (.ref .bool) := by
+  intros Γ t1 t2 hsem st1 st2 m Δ1 Δ2 wf1 wf2 henv hst
+  have hexp := hsem st1 st2 m Δ1 Δ2 wf1 wf2 henv hst
+  rcases hexp with ⟨st1', st2', m', v1, v2, hm1, hstore, hstep1, hstep2, hcl1, hcl2, hv12⟩
+  have hm2 := extend.ext st1' st2' m' hstore
+  have hm3 := extend.trans hm1 hm2
+  exists (v1::st1'), (v2::st2'), (st_rel.ext m' st1'.length st2'.length),
+         (.loc st1'.length), (.loc st2'.length);
+  constructor; apply hm3
+  constructor; apply storeType.ext; assumption; assumption
+  simp; constructor; apply stepnTrans; apply stepnRef; apply hstep1
+  apply stepnRefVal; exact (valTypeValue _ _ _ _ hv12).1
+  apply stepnTrans; apply stepnRef; apply hstep2
+  apply stepnRefVal; exact (valTypeValue _ _ _ _ hv12).2
+
+lemma semDeref : ∀ Γ t1 t2,
+  semType Γ t1 t2 (.ref .bool) →
+  semType Γ (.deref t1) (.deref t2) .bool := by sorry
+
+lemma semAssign : ∀ Γ t1 t2 t1' t2',
+  semType Γ t1 t1' (.ref .bool) →
+  semType Γ t2 t2' .bool →
+  semType Γ (.assign t1 t2) (.assign t1' t2') .bool := by sorry
+
+lemma semApp : ∀ Γ f1 f2 t1 t2 τ1 τ2,
+  semType Γ f1 f2 (.arrow τ1 τ2) →
+  semType Γ t1 t2 τ1 →
+  semType Γ (.app f1 t1) (.app f2 t2) τ2 := by sorry
